examples/pkc_checker/array/compilation/scpogCompileScript.sml
@@ -1,0 +1,16 @@
+(*
+  Compiles the scpog example by evaluation inside the logic of HOL
+*)
+open preamble scpog_arrayFullProgTheory eval_cake_compile_x64Lib
+open fromSexpTheory astToSexprLib
+
+val _ = new_theory "scpogCompile"
+
+(*
+val _ = astToSexprLib.write_ast_to_file "cake_scpog.sexp" prog;
+*)
+
+Theorem scpog_array_compiled =
+  eval_cake_compile_x64 "" main_prog_def "cake_scpog.S";
+
+val _ = export_theory ();
